Veir/Rewriter/GetSet/BlockArguments.lean
@@ -1,0 +1,435 @@
+module
+
+public import Veir.Rewriter.Basic
+
+import all Veir.Rewriter.Basic
+
+public section
+
+/-
+ - The getters we consider are:
+ - * BlockPtr.get! optionally replaced by the following special cases:
+ -   * Block.firstUse
+ -   * Block.prev
+ -   * Block.next
+ -   * Block.parent
+ -   * Block.firstOp
+ -   * Block.lastOp
+ - * OperationPtr.get! optionally replaced by the following special cases:
+ -   * Operation.prev
+ -   * Operation.next
+ -   * Operation.parent
+ -   * OperationPtr.getOpType!
+ -   * Operation.attrs
+ - * OperationPtr.getProperties!
+ - * OperationPtr.getNumResults!
+ - * OpResultPtr.get!
+ - * OperationPtr.getNumOperands!
+ - * OpOperandPtr.get! optionally replaced by the following special case:
+ - * OperationPtr.getOperands!
+ - * OperationPtr.getNumSuccessors!
+ - * BlockOperandPtr.get!
+ - * OperationPtr.getSuccessor!
+ - * OperationPtr.getSuccessors!
+ - * OperationPtr.getNumRegions!
+ - * OperationPtr.getRegion!
+ - * BlockOperandPtrPtr.get!
+ - * BlockPtr.getNumArguments!
+ - * BlockArgumentPtr.get!
+ - * RegionPtr.get! with optionally special cases for:
+ -   * firstBlock
+ -   * lastBlock
+ -   * parent
+ - * ValuePtr.getFirstUse!
+ - * ValuePtr.getType!
+ - * OpOperandPtrPtr.get!
+ -/
+
+namespace Veir
+
+variable {OpInfo} [HasOpInfo OpInfo]
+variable {ctx : IRContext OpInfo}
+
+/-! ## `Rewriter.pushBlockArgument` -/
+
+section Rewriter.pushBlockArgument
+
+variable {block : BlockPtr}
+
+attribute [local grind] Rewriter.pushBlockArgument
+
+@[simp, grind =]
+theorem BlockPtr.firstUse!_Rewriter_pushBlockArgument {block' : BlockPtr} :
+    (block'.get! (Rewriter.pushBlockArgument ctx block type hblock)).firstUse =
+    (block'.get! ctx).firstUse := by
+  grind
+
+@[simp, grind =]
+theorem BlockPtr.prev!_Rewriter_pushBlockArgument {block' : BlockPtr} :
+    (block'.get! (Rewriter.pushBlockArgument ctx block type hblock)).prev =
+    (block'.get! ctx).prev := by
+  grind
+
+@[simp, grind =]
+theorem BlockPtr.next!_Rewriter_pushBlockArgument {block' : BlockPtr} :
+    (block'.get! (Rewriter.pushBlockArgument ctx block type hblock)).next =
+    (block'.get! ctx).next := by
+  grind
+
+@[simp, grind =]
+theorem BlockPtr.parent!_Rewriter_pushBlockArgument {block' : BlockPtr} :
+    (block'.get! (Rewriter.pushBlockArgument ctx block type hblock)).parent =
+    (block'.get! ctx).parent := by
+  grind
+
+@[simp, grind =]
+theorem BlockPtr.firstOp!_Rewriter_pushBlockArgument {block' : BlockPtr} :
+    (block'.get! (Rewriter.pushBlockArgument ctx block type hblock)).firstOp =
+    (block'.get! ctx).firstOp := by
+  grind
+
+@[simp, grind =]
+theorem BlockPtr.lastOp!_Rewriter_pushBlockArgument {block' : BlockPtr} :
+    (block'.get! (Rewriter.pushBlockArgument ctx block type hblock)).lastOp =
+    (block'.get! ctx).lastOp := by
+  grind
+
+@[simp, grind =]
+theorem OperationPtr.get!_Rewriter_pushBlockArgument {operation : OperationPtr} :
+    operation.get! (Rewriter.pushBlockArgument ctx block type hblock) =
+    operation.get! ctx := by
+  grind
+
+@[simp, grind =]
+theorem OperationPtr.getOpType!_Rewriter_pushBlockArgument {operation : OperationPtr} :
+    operation.getOpType! (Rewriter.pushBlockArgument ctx block type hblock) =
+    operation.getOpType! ctx := by
+  grind
+
+@[simp, grind =]
+theorem OperationPtr.getProperties!_Rewriter_pushBlockArgument {operation : OperationPtr} :
+    operation.getProperties! (Rewriter.pushBlockArgument ctx block type hblock) opCode =
+    operation.getProperties! ctx opCode := by
+  grind
+
+@[simp, grind =]
+theorem OperationPtr.getNumResults!_Rewriter_pushBlockArgument {operation : OperationPtr} :
+    operation.getNumResults! (Rewriter.pushBlockArgument ctx block type hblock) =
+    operation.getNumResults! ctx := by
+  grind
+
+@[simp, grind =]
+theorem OpResultPtr.get!_Rewriter_pushBlockArgument {opResult : OpResultPtr} :
+    opResult.get! (Rewriter.pushBlockArgument ctx block type hblock) =
+    opResult.get! ctx := by
+  grind
+
+@[simp, grind =]
+theorem OperationPtr.getNumOperands!_Rewriter_pushBlockArgument {operation : OperationPtr} :
+    operation.getNumOperands! (Rewriter.pushBlockArgument ctx block type hblock) =
+    operation.getNumOperands! ctx := by
+  grind
+
+@[simp, grind =]
+theorem OpOperandPtr.get!_Rewriter_pushBlockArgument {opOperand : OpOperandPtr} :
+    opOperand.get! (Rewriter.pushBlockArgument ctx block type hblock) =
+    opOperand.get! ctx := by
+  grind
+
+@[simp, grind =]
+theorem OperationPtr.getOperands!_Rewriter_pushBlockArgument {operation : OperationPtr} :
+    operation.getOperands! (Rewriter.pushBlockArgument ctx block type hblock) =
+    operation.getOperands! ctx := by
+  grind
+
+@[simp, grind =]
+theorem OperationPtr.getNumSuccessors!_Rewriter_pushBlockArgument {operation : OperationPtr} :
+    operation.getNumSuccessors! (Rewriter.pushBlockArgument ctx block type hblock) =
+    operation.getNumSuccessors! ctx := by
+  grind
+
+@[simp, grind =]
+theorem BlockOperandPtr.get!_Rewriter_pushBlockArgument {blockOperand : BlockOperandPtr} :
+    blockOperand.get! (Rewriter.pushBlockArgument ctx block type hblock) =
+    blockOperand.get! ctx := by
+  grind
+
+@[simp, grind =]
+theorem OperationPtr.getSuccessor!_Rewriter_pushBlockArgument {operation : OperationPtr} :
+    operation.getSuccessor! (Rewriter.pushBlockArgument ctx block type hblock) index =
+    operation.getSuccessor! ctx index := by
+  grind [OperationPtr.getSuccessor!_def]
+
+@[simp, grind =]
+theorem OperationPtr.getSuccessors!_Rewriter_pushBlockArgument {operation : OperationPtr} :
+    operation.getSuccessors! (Rewriter.pushBlockArgument ctx block type hblock) =
+    operation.getSuccessors! ctx := by
+  grind [OperationPtr.getSuccessors!_def]
+
+@[simp, grind =]
+theorem OperationPtr.getNumRegions!_Rewriter_pushBlockArgument {operation : OperationPtr} :
+    operation.getNumRegions! (Rewriter.pushBlockArgument ctx block type hblock) =
+    operation.getNumRegions! ctx := by
+  grind
+
+@[simp, grind =]
+theorem OperationPtr.getRegion!_Rewriter_pushBlockArgument {operation : OperationPtr} :
+    operation.getRegion! (Rewriter.pushBlockArgument ctx block type hblock) idx =
+    operation.getRegion! ctx idx := by
+  grind
+
+@[simp, grind =]
+theorem BlockOperandPtrPtr.get!_Rewriter_pushBlockArgument {blockOperandPtr : BlockOperandPtrPtr} :
+    blockOperandPtr.get! (Rewriter.pushBlockArgument ctx block type hblock) =
+    blockOperandPtr.get! ctx := by
+  grind
+
+@[grind =]
+theorem BlockPtr.getNumArguments!_Rewriter_pushBlockArgument {block' : BlockPtr} :
+    block'.getNumArguments! (Rewriter.pushBlockArgument ctx block type hblock) =
+    if block = block' then
+      block'.getNumArguments! ctx + 1
+    else
+      block'.getNumArguments! ctx := by
+  grind
+
+@[grind =]
+theorem BlockArgumentPtr.get!_Rewriter_pushBlockArgument {blockArg : BlockArgumentPtr} :
+    blockArg.get! (Rewriter.pushBlockArgument ctx block type hblock) =
+    if blockArg = block.nextArgument ctx then
+      { type := type, firstUse := none, index := block.getNumArguments! ctx, owner := block, loc := ()}
+    else
+      blockArg.get! ctx := by
+  grind
+
+@[simp, grind =]
+theorem RegionPtr.get!_Rewriter_pushBlockArgument {region : RegionPtr} :
+    region.get! (Rewriter.pushBlockArgument ctx block type hblock) =
+    region.get! ctx := by
+  grind
+
+@[grind =]
+theorem ValuePtr.getFirstUse!_Rewriter_pushBlockArgument {value : ValuePtr} :
+    value.getFirstUse! (Rewriter.pushBlockArgument ctx block type hblock) =
+    if value = block.nextArgument ctx then
+      none
+    else
+      value.getFirstUse! ctx := by
+  grind
+
+@[grind =]
+theorem ValuePtr.getType!_Rewriter_pushBlockArgument {value : ValuePtr} :
+    value.getType! (Rewriter.pushBlockArgument ctx block type hblock) =
+    if value = block.nextArgument ctx then
+      type
+    else
+      value.getType! ctx := by
+  grind
+
+@[grind =]
+theorem OpOperandPtrPtr.get!_Rewriter_pushBlockArgument {opOperandPtr : OpOperandPtrPtr} :
+    opOperandPtr.get! (Rewriter.pushBlockArgument ctx block type hblock) =
+    if opOperandPtr = OpOperandPtrPtr.valueFirstUse (block.nextArgument ctx) then
+      none
+    else
+      opOperandPtr.get! ctx := by
+  grind
+
+end Rewriter.pushBlockArgument
+
+/-! ## `Rewriter.initBlockArguments` -/
+
+section Rewriter.initBlockArguments
+
+variable {op : OperationPtr}
+
+attribute [local grind] Rewriter.initBlockArguments
+
+@[simp, grind =]
+theorem BlockPtr.firstUse!_initBlockArguments {block' : BlockPtr} :
+    (block'.get! (Rewriter.initBlockArguments ctx block types idx h₁ h₂)).firstUse =
+    (block'.get! ctx).firstUse := by
+  fun_induction Rewriter.initBlockArguments <;> grind
+
+@[simp, grind =]
+theorem BlockPtr.prev!_initBlockArguments {block' : BlockPtr} :
+    (block'.get! (Rewriter.initBlockArguments ctx block types idx h₁ h₂)).prev =
+    (block'.get! ctx).prev := by
+  fun_induction Rewriter.initBlockArguments <;> grind
+
+@[simp, grind =]
+theorem BlockPtr.next!_initBlockArguments {block' : BlockPtr} :
+    (block'.get! (Rewriter.initBlockArguments ctx block types idx h₁ h₂)).next =
+    (block'.get! ctx).next := by
+  fun_induction Rewriter.initBlockArguments <;> grind
+
+@[simp, grind =]
+theorem BlockPtr.parent!_initBlockArguments {block' : BlockPtr} :
+    (block'.get! (Rewriter.initBlockArguments ctx block types idx h₁ h₂)).parent =
+    (block'.get! ctx).parent := by
+  fun_induction Rewriter.initBlockArguments <;> grind
+
+@[simp, grind =]
+theorem BlockPtr.firstOp!_initBlockArguments {block' : BlockPtr} :
+    (block'.get! (Rewriter.initBlockArguments ctx block types idx h₁ h₂)).firstOp =
+    (block'.get! ctx).firstOp := by
+  fun_induction Rewriter.initBlockArguments <;> grind
+
+@[simp, grind =]
+theorem BlockPtr.lastOp!_initBlockArguments {block' : BlockPtr} :
+    (block'.get! (Rewriter.initBlockArguments ctx block types idx h₁ h₂)).lastOp =
+    (block'.get! ctx).lastOp := by
+  fun_induction Rewriter.initBlockArguments <;> grind
+
+@[simp, grind =]
+theorem OperationPtr.get!_initBlockArguments {operation : OperationPtr} :
+    operation.get! (Rewriter.initBlockArguments ctx block types idx h₁ h₂) =
+    operation.get! ctx := by
+  fun_induction Rewriter.initBlockArguments <;> grind
+
+@[simp, grind =]
+theorem OperationPtr.getOpType!_initBlockArguments {operation : OperationPtr} :
+    operation.getOpType! (Rewriter.initBlockArguments ctx block types idx h₁ h₂) =
+    operation.getOpType! ctx := by
+  fun_induction Rewriter.initBlockArguments <;> grind
+
+@[simp, grind =]
+theorem OperationPtr.getProperties!_initBlockArguments {operation : OperationPtr} :
+    operation.getProperties! (Rewriter.initBlockArguments ctx block types idx h₁ h₂) opCode =
+    operation.getProperties! ctx opCode := by
+  fun_induction Rewriter.initBlockArguments <;> grind
+
+@[simp, grind =]
+theorem OperationPtr.getNumResults!_initBlockArguments {operation : OperationPtr} :
+    operation.getNumResults! (Rewriter.initBlockArguments ctx block types idx h₁ h₂) =
+    operation.getNumResults! ctx := by
+  fun_induction Rewriter.initBlockArguments <;> grind
+
+@[simp, grind =]
+theorem OpResultPtr.get!_initBlockArguments {opResult : OpResultPtr} :
+    opResult.get! (Rewriter.initBlockArguments ctx block types idx h₁ h₂) =
+    opResult.get! ctx := by
+  fun_induction Rewriter.initBlockArguments <;> grind [cases OpResultPtr]
+
+@[simp, grind =]
+theorem OperationPtr.getNumOperands!_initBlockArguments {operation : OperationPtr} :
+    operation.getNumOperands! (Rewriter.initBlockArguments ctx block types idx h₁ h₂) =
+    operation.getNumOperands! ctx := by
+  fun_induction Rewriter.initBlockArguments <;> grind
+
+@[simp, grind =]
+theorem OpOperandPtr.get!_initBlockArguments {opOperand : OpOperandPtr}:
+    opOperand.get! (Rewriter.initBlockArguments ctx block types idx h₁ h₂) = opOperand.get! ctx := by
+  fun_induction Rewriter.initBlockArguments <;> grind
+
+@[simp, grind =]
+theorem OperationPtr.getOperands!_initBlockArguments {operation : OperationPtr} :
+    operation.getOperands! (Rewriter.initBlockArguments ctx block types idx h₁ h₂) = operation.getOperands! ctx := by
+  fun_induction Rewriter.initBlockArguments <;> grind
+
+@[simp, grind =]
+theorem OperationPtr.getNumSuccessors!_initBlockArguments {operation : OperationPtr} :
+    operation.getNumSuccessors! (Rewriter.initBlockArguments ctx block types idx h₁ h₂) =
+    operation.getNumSuccessors! ctx := by
+  fun_induction Rewriter.initBlockArguments <;> grind
+
+@[simp, grind =]
+theorem BlockOperandPtr.get!_initBlockArguments {blockOperand : BlockOperandPtr} :
+    blockOperand.get! (Rewriter.initBlockArguments ctx block types idx h₁ h₂) =
+    blockOperand.get! ctx := by
+  fun_induction Rewriter.initBlockArguments <;> grind
+
+@[simp, grind =]
+theorem OperationPtr.getSuccessor!_initBlockArguments {operation : OperationPtr} :
+    operation.getSuccessor! (Rewriter.initBlockArguments ctx block types idx h₁ h₂) i =
+    operation.getSuccessor! ctx i := by
+  fun_induction Rewriter.initBlockArguments <;> grind [OperationPtr.getSuccessor!_def]
+
+@[simp, grind =]
+theorem OperationPtr.getSuccessors!_initBlockArguments {operation : OperationPtr} :
+    operation.getSuccessors! (Rewriter.initBlockArguments ctx block types idx h₁ h₂) =
+    operation.getSuccessors! ctx := by
+  simp only [OperationPtr.getSuccessors!_def, OperationPtr.getSuccessor!_initBlockArguments,
+    OperationPtr.getNumSuccessors!_initBlockArguments]
+
+@[simp, grind =]
+theorem OperationPtr.getNumRegions!_initBlockArguments {operation : OperationPtr} :
+    operation.getNumRegions! (Rewriter.initBlockArguments ctx block types idx h₁ h₂) =
+    operation.getNumRegions! ctx := by
+  fun_induction Rewriter.initBlockArguments <;> grind
+
+@[simp, grind =]
+theorem OperationPtr.getRegion!_initBlockArguments {operation : OperationPtr} :
+    operation.getRegion! (Rewriter.initBlockArguments ctx block types index h₁ h₂) idx =
+    operation.getRegion! ctx idx := by
+  fun_induction Rewriter.initBlockArguments <;> grind
+
+@[simp, grind =]
+theorem BlockOperandPtrPtr.get!_initBlockArguments {blockOperandPtr : BlockOperandPtrPtr} :
+    blockOperandPtr.get! (Rewriter.initBlockArguments ctx block types idx h₁ h₂) =
+    blockOperandPtr.get! ctx := by
+  fun_induction Rewriter.initBlockArguments <;> grind
+
+@[grind =]
+theorem BlockPtr.getNumArguments!_initBlockArguments {block' : BlockPtr} :
+    block'.getNumArguments! (Rewriter.initBlockArguments ctx block types idx h₁ h₂) =
+    if block = block' then
+      block'.getNumArguments! ctx + (types.size - idx)
+    else
+      block'.getNumArguments! ctx := by
+  fun_induction Rewriter.initBlockArguments <;> grind
+
+@[grind =]
+theorem BlockArgumentPtr.get!_initBlockArguments {blockArg : BlockArgumentPtr} :
+    blockArg.get! (Rewriter.initBlockArguments ctx bl types idx h₁ h₂) =
+    if h : blockArg.block = bl ∧ blockArg.index < types.size ∧ bl.getNumArguments! ctx ≤ blockArg.index then
+      { type := types[blockArg.index], firstUse := none, index := blockArg.index, owner := bl, loc := ()}
+    else blockArg.get! ctx := by
+  fun_induction Rewriter.initBlockArguments <;> grind [BlockPtr.getArgument_def, cases BlockArgumentPtr]
+
+@[simp, grind =]
+theorem RegionPtr.get!_initBlockArguments {region : RegionPtr} :
+    region.get! (Rewriter.initBlockArguments ctx block types idx h₁ h₂) =
+    region.get! ctx := by
+  fun_induction Rewriter.initBlockArguments <;> grind
+
+@[grind =]
+theorem ValuePtr.getFirstUse!_initBlockArguments {value : ValuePtr} :
+    value.getFirstUse! (Rewriter.initBlockArguments ctx block types idx h₁ h₂) =
+    match value with
+    | .blockArgument blockArg =>
+      if blockArg.block = block ∧ blockArg.index < types.size ∧ block.getNumArguments! ctx ≤ blockArg.index then
+        none
+      else value.getFirstUse! ctx
+    | _ => value.getFirstUse! ctx := by
+  fun_induction Rewriter.initBlockArguments <;>
+    grind [cases BlockArgumentPtr, cases ValuePtr, BlockPtr.getArgument_def]
+
+@[grind =]
+theorem ValuePtr.getType!_initBlockArguments {value : ValuePtr} :
+    value.getType! (Rewriter.initBlockArguments ctx block types idx h₁ h₂) =
+    match value with
+    | .blockArgument blockArg =>
+      if _ : blockArg.block = block ∧ blockArg.index < types.size ∧ block.getNumArguments! ctx ≤ blockArg.index then
+        types[blockArg.index]
+      else value.getType! ctx
+    | _ => value.getType! ctx := by
+  fun_induction Rewriter.initBlockArguments <;>
+    grind [cases BlockArgumentPtr, cases ValuePtr, BlockPtr.getArgument_def]
+
+@[grind =]
+theorem OpOperandPtrPtr.get!_initBlockArguments {opOperandPtr : OpOperandPtrPtr} :
+    opOperandPtr.get! (Rewriter.initBlockArguments ctx block types idx h₁ h₂) =
+    match opOperandPtr with
+    | .valueFirstUse (.blockArgument blockArg) =>
+      if _ : blockArg.block = block ∧ blockArg.index < types.size ∧ block.getNumArguments! ctx ≤ blockArg.index then
+        none
+      else (blockArg.get! ctx).firstUse
+    | _ => opOperandPtr.get! ctx := by
+  cases opOperandPtr
+  · grind
+  · simp only [get!_valueFirstUse_eq, ValuePtr.getFirstUse!_initBlockArguments, dite_eq_ite]; grind
+
+end Rewriter.initBlockArguments
+
+end Veir
