Veir/Rewriter/WellFormed/BlockArguments.lean
@@ -1,0 +1,91 @@
+module
+
+public import Veir.IR.Basic
+public import Veir.Rewriter.Basic
+
+import all Veir.Rewriter.Basic
+import Veir.IR.WellFormed
+import Veir.Rewriter.GetSet
+
+public section
+
+namespace Veir
+
+variable {OpInfo : Type} [HasOpInfo OpInfo]
+variable {ctx : IRContext OpInfo}
+
+/-! ## Rewriter.pushBlockArgument -/
+
+theorem BlockPtr.opChain_Rewriter_pushBlockArgument
+    (hWf : BlockPtr.OpChain block' ctx array) :
+    BlockPtr.OpChain block' (Rewriter.pushBlockArgument ctx block type hblock) array := by
+  apply BlockPtr.OpChain_unchanged (ctx := ctx) <;> grind
+
+theorem ValuePtr.defUse_Rewriter_pushBlockArgument
+    (hWf : ValuePtr.DefUse value ctx array missingUses) :
+    ValuePtr.DefUse value (Rewriter.pushBlockArgument ctx block type hblock) array missingUses := by
+  apply ValuePtr.DefUse.unchanged (ctx := ctx) <;> grind
+
+theorem ValuePtr.defUse_Rewriter_pushBlockArgument_newResult (ctxFIB : ctx.FieldsInBounds) :
+    ValuePtr.DefUse (block.nextArgument ctx) (Rewriter.pushBlockArgument ctx block type hblock) #[] ∅ := by
+  constructor <;> grind
+
+theorem BlockPtr.defUse_Rewriter_pushBlockArgument
+    (hWf : BlockPtr.DefUse block' ctx array missingUses) :
+    BlockPtr.DefUse block' (Rewriter.pushBlockArgument ctx block type hblock) array missingUses := by
+  apply BlockPtr.DefUse.unchanged (ctx := ctx) <;> grind
+
+theorem RegionPtr.blockChain_Rewriter_pushBlockArgument
+    (hWf : RegionPtr.BlockChain region ctx array) :
+    RegionPtr.BlockChain region (Rewriter.pushBlockArgument ctx block type hblock) array := by
+  apply RegionPtr.blockChain_unchanged (ctx := ctx) hWf <;> grind
+
+theorem IRContext.wellFormed_Rewriter_pushBlockArgument :
+    ctx.WellFormed →
+    (Rewriter.pushBlockArgument ctx block type hblock).WellFormed := by
+  intro wf
+  have ⟨h₁, h₂, h₃, h₄, h₅, h₆, h₇, h₈⟩ := wf
+  constructor
+  case inBounds => grind
+  case valueDefUseChains =>
+    intros val hval
+    have valCases : val.InBounds ctx ∨ val = block.nextArgument ctx := by grind
+    cases valCases
+    case inl valInBounds =>
+      have ⟨array, harray⟩ := h₂ val (by grind)
+      exists array
+      grind [ValuePtr.defUse_Rewriter_pushBlockArgument]
+    case inr hvalEq =>
+      grind [ValuePtr.defUse_Rewriter_pushBlockArgument_newResult]
+  case blockDefUseChains =>
+    intros block hblock
+    have ⟨array, harray⟩ := h₃ block (by grind)
+    exists array
+    grind [BlockPtr.defUse_Rewriter_pushBlockArgument]
+  case opChain =>
+    intros block' hBlock'
+    have ⟨array', harray'⟩ := h₄ block' (by grind)
+    exists array'
+    grind [BlockPtr.opChain_Rewriter_pushBlockArgument]
+  case blockChain =>
+    intros region hregion
+    have ⟨array, harray⟩ := h₅ region (by grind)
+    exists array
+    apply RegionPtr.blockChain_unchanged harray <;> grind
+  case operations =>
+    intros op' hop'
+    apply OperationPtr.WellFormed_unchanged (ctx := ctx) <;> grind
+  case blocks =>
+    intros bl hbl
+    have : bl.InBounds ctx := by grind
+    have ⟨ha, hb, hc, hd, he⟩ := h₇ bl (by grind)
+    constructor <;> grind
+  case regions =>
+    grind [RegionPtr.WellFormed_unchanged]
+
+/-! ## Rewriter.initBlockArguments -/
+
+theorem IRContext.wellFormed_Rewriter_initBlockArguments :
+    ctx.WellFormed →
+    (Rewriter.initBlockArguments ctx opPtr resultTypes index hop hindex).WellFormed := by
+  fun_induction Rewriter.initBlockArguments <;> grind [IRContext.wellFormed_Rewriter_pushBlockArgument]
